compiler1/semantics/stackSemScript.sml
@@ -310,7 +310,7 @@ val evaluate_def = tDefine "evaluate" `
        if res = NONE then evaluate (c2,check_clock s1 s) else (res,s1)) /\
   (evaluate (Return n m,s) =
      case (get_var n s ,get_var m s) of
-     | (SOME x,SOME y) => (SOME (Result x y),empty_env s)
+     | (SOME x,SOME y) => (SOME (Result x y),s)
      | _ => (SOME Error,s)) /\
   (evaluate (Raise n,s) =
      case get_var n s of
