compiler1/semantics/wordSemScript.sml
@@ -184,11 +184,11 @@ val key_val_compare_def = Define `
   key_val_compare x y =
     let (a:num,b) = x in
     let (a':num,b') = y in
-      (a < a') \/
+      (a > a') \/
       (a = a' /\
         case b of
           Word x => (case b' of Word y => x <= y | _ => T)
-        | Loc a b => case b' of Loc a' b' => (a<a') \/ (a=a' /\ b<=b') | _ => F)`
+        | Loc a b => case b' of Loc a' b' => (a>a') \/ (a=a' /\ b>=b') | _ => F)`
 
 (*
 EVAL ``key_val_compare (1,Loc 3 4) (1,Loc 1 2)``
